src/dice_engine/DICE.Engine.Definitions.fst
@@ -14,8 +14,6 @@ open Lib.IntTypes
  * Some common definitions used in the DICE code
  *)
 
-#set-options "--__temp_no_proj DICE.Definitions"
-
 let byte_sec = uint8
 let byte_pub = pub_uint8
 
@@ -25,8 +23,10 @@ let bytes_pub = Seq.seq I.pub_uint8
 let lbytes_sec = Seq.lseq I.uint8
 let lbytes_pub = Seq.lseq I.pub_uint8
 
-type dice_hash_alg = a:S.hash_alg{
-  a =!= S.MD5 /\ a =!= S.SHA2_224 /\ a =!= S.Blake2S /\ a =!= S.Blake2B
+type dice_hash_alg = a:S.hash_alg {
+  a =!= S.MD5 /\ a =!= S.SHA2_224 /\ a =!= S.Blake2S /\ a =!= S.Blake2B /\ a =!= S.SHA1 /\
+  (not (S.is_shake a)) /\
+  Some? (S.max_input_length a)
 }
 
 inline_for_extraction
@@ -35,10 +35,9 @@ let alg : dice_hash_alg = S.SHA2_256
 inline_for_extraction noextract
 let dice_hash (alg:dice_hash_alg) : H.hash_st alg =
   match alg with
-  | S.SHA2_256 -> Hacl.Hash.SHA2.hash_256
-  | S.SHA2_384 -> Hacl.Hash.SHA2.hash_384
-  | S.SHA2_512 -> Hacl.Hash.SHA2.hash_512
-  | S.SHA1     -> Hacl.Hash.SHA1.legacy_hash
+  | S.SHA2_256 -> Hacl.Streaming.SHA2.hash_256
+  | S.SHA2_384 -> Hacl.Streaming.SHA2.hash_384
+  | S.SHA2_512 -> Hacl.Streaming.SHA2.hash_512
 
 inline_for_extraction noextract
 let dice_hmac (alg:dice_hash_alg) : Hacl.HMAC.compute_st alg =
@@ -46,13 +45,12 @@ let dice_hmac (alg:dice_hash_alg) : Hacl.HMAC.compute_st alg =
   | S.SHA2_256 -> Hacl.HMAC.compute_sha2_256
   | S.SHA2_384 -> Hacl.HMAC.compute_sha2_384
   | S.SHA2_512 -> Hacl.HMAC.compute_sha2_512
-  | S.SHA1     -> Hacl.HMAC.legacy_compute_sha1
 
 unfold let digest_len = H.hash_len alg
 
 unfold type digest_t = H.hash_t alg
 
-unfold type hashable_len = i: size_t {0 < v i /\ v i <= S.max_input_length alg}
+unfold type hashable_len = i: size_t {0 < v i /\ v i <= (Some?.v (S.max_input_length alg))}
 unfold type signable_len = i: size_t {64 + v i <= max_size_t}
 unfold let cdi_len = digest_len
 
