src/l0/L0.X509.AliasKeyTBS.Extensions.fst
@@ -19,8 +19,6 @@ module P = FStar.Pervasives
 
 #set-options "--z3rlimit 128 --fuel 0 --ifuel 0 --using_facts_from '* -FStar.Tactics -FStar.Reflection'"
 
-#set-options "--__temp_no_proj L0.X509.AliasKeyTBS.Extensions"
-
 let decl = ()
 
 
