src/l0/L0.X509.Base.fst
@@ -5,8 +5,6 @@ open X509
 
 module B32 = FStar.Bytes
 
-#set-options "--__temp_no_proj L0.X509.Base"
-
 noeq
 type deviceIDCSR_ingredients_t = {
   deviceIDCSR_ku: key_usage_payload_t;
