src/l0/L0.X509.DeviceIDCRI.fst
@@ -11,8 +11,6 @@ module B32 = FStar.Bytes
 
 #set-options "--z3rlimit 256 --fuel 0 --ifuel 0"
 
-#set-options "--__temp_no_proj L0.X509.DeviceIDCRI"
-
 let decl = ()
 
 (*     (To-Be-Signed) DeviceID Certification Request Info
